ironfleet/src/Dafny/Distributed/Common/Framework/Performance.s.dfy
@@ -25,7 +25,8 @@ abstract module Performance_s {
 
     ensures p1.PerfAdd? && PerfVoid in p1.prs && p2 == PerfZero ==> PerfEq(p1, p2)
     ensures p1.PerfAdd? && p2 == PerfAdd(p1.prs[PerfZero() := 0]) ==> PerfEq(p1, p2)
-
+    ensures p1.PerfAdd? && p1.prs == multiset{} && p2 == PerfZero ==> PerfEq(p1, p2)
+    ensures p2.PerfAdd? && p2.prs == multiset{} && p1 == PerfZero ==> PerfEq(p1, p2)
 
     // Want to establish associativity
     // PerfAdd(multiset{PerfAdd(p1), prs'}) == PerfAdd(p1 + prs')
