ironfleet/src/Dafny/Distributed/Protocol/Lock/PerformanceProof/Definitions.i.dfy
@@ -6,18 +6,18 @@ import opened LockTaggedDistributedSystem_i
   // import opened TaggedGLS_i
 
 function PerfBoundLockHeld(epoch: int) : PerfReport
-  requires 0 <= epoch
+  requires 0 < epoch
 {
   var s : multiset<PerformanceReport> := multiset{};
-  var s2 := s[PerfStep(GrantStep) := epoch][PerfStep(AcceptStep) := epoch];
+  var s2 := s[PerfStep(GrantStep) := epoch - 1][PerfStep(AcceptStep) := epoch - 1];
   PerfAdd(s2)
 }
 
 function PerfBoundLockInNetwork(epoch: int) : PerfReport
-  requires 0 < epoch
+  requires 1 < epoch
 {
   var s : multiset<PerformanceReport> := multiset{};
-  var s2 := s[PerfStep(GrantStep) := epoch][PerfStep(AcceptStep) := epoch - 1];
+  var s2 := s[PerfStep(GrantStep) := epoch - 1][PerfStep(AcceptStep) := epoch - 2];
   PerfAdd(s2)
 }
 
